cklr/InjectUnusedglob.v
@@ -1,0 +1,174 @@
+Require Import Axioms.
+Require Import Events.
+Require Import CallconvAlgebra.
+Require Import CKLR.
+Require Import CKLRAlgebra.
+Require Import LanguageInterface.
+
+Require Import Inject.
+
+Record inj_stbls' (w: inj_world) (se1 se2: Genv.symtbl): Prop :=
+  {
+    inj_stbls_match: Genv.match_stbls' (injw_meminj w) se1 se2;
+    inj_stbls_next_l: Pos.le (Genv.genv_next se1) (injw_next_l w);
+    inj_stbls_next_r: Pos.le (Genv.genv_next se2) (injw_next_r w);
+  }.
+
+Global Instance inj_stbls_subrel':
+  Monotonic inj_stbls' (inj_incr ++> subrel).
+Proof.
+  intros w w' Hw se1 se2 Hse.
+  destruct Hse; inv Hw. cbn in *.
+  constructor; cbn; try extlia.
+  eapply Genv.match_stbls_incr'; eauto.
+  intros. edestruct H0; eauto. extlia.
+Qed.
+
+Program Definition inj' : cklr :=
+  {|
+    world := inj_world;
+    wacc := inj_incr;
+    mi := injw_meminj;
+    match_stbls := inj_stbls';
+    match_mem := inj_mem;
+  |}.
+
+Next Obligation. (* mi_acc_separated *)
+  eapply inj_acc_separated; eauto.
+Qed.
+
+Next Obligation.
+Admitted.
+(* TODO: relax this requirement of cklr *)
+
+
+Next Obligation.
+  destruct H. inv H0; cbn in *. extlia.
+Qed.
+
+Next Obligation. (* Mem.alloc *)
+  exact inj_cklr_alloc.
+Qed.
+
+
+Next Obligation. (* Mem.free *)
+  intros [f nb1 nb2] m1 m2 Hm [[b1 lo1] hi1] [[b2 lo2] hi2] Hr.
+  simpl. red.
+  destruct (Mem.free m1 b1 lo1 hi1) as [m1'|] eqn:Hm1'; [|rauto].
+  inv Hr. cbn in H0. inv H0. inv Hm.
+  edestruct Mem.free_parallel_inject as (m2' & Hm2' & Hm'); eauto.
+  replace (lo1 + delta + sz) with (lo1 + sz + delta) by extlia.
+  rewrite Hm2'.
+  repeat (econstructor; eauto); try congruence;
+    erewrite <- Mem.nextblock_free; eauto using Pos.le_refl.
+Qed.
+
+Next Obligation. (* Mem.load *)
+  intros [f nb1 nb2] chunk m1 m2 Hm _ _ [b1 ofs1 b2 delta Hptr].
+  cbn in *. red. inv Hm.
+  destruct (Mem.load chunk m1 b1 ofs1) as [v1|] eqn:Hv1; [|rauto].
+  edestruct Mem.load_inject as (v2 & Hv2 & Hv); eauto.
+  rewrite Hv2. repeat (econstructor; eauto).
+Qed.
+
+Next Obligation. (* Mem.store *)
+  intros [f nb1 nb2] chunk m1 m2 Hm _ _ [b1 ofs1 b2 delta Hptr] v1 v2 Hv.
+  red in Hv |- *. cbn in *. inv Hm.
+  destruct (Mem.store chunk m1 b1 ofs1 v1) as [m1'|] eqn:Hm1'; [|rauto].
+  edestruct Mem.store_mapped_inject as (m2' & Hm2' & Hm'); eauto.
+  rewrite Hm2'.
+  repeat (econstructor; eauto); try congruence;
+    erewrite <- Mem.nextblock_store; eauto using Pos.le_refl.
+Qed.
+
+Next Obligation. (* Mem.loadbytes *)
+  intros [f nb1 nb2] m1 m2 Hm _ _ [b1 ofs1 b2 delta Hptr] sz.
+  red. cbn in *. inv Hm.
+  destruct (Mem.loadbytes m1 b1 ofs1 sz) as [vs1|] eqn:Hvs1; [|rauto].
+  edestruct Mem.loadbytes_inject as (vs2 & Hvs2 & Hvs); eauto.
+  rewrite Hvs2. rauto.
+Qed.
+
+Next Obligation. (* Mem.storebytes *)
+  intros [f nb1 nb2] m1 m2 Hm [b1 ofs1] [b2 ofs2] Hptr vs1 vs2 Hvs.
+  red in Hvs |- *. cbn in *. inv Hm.
+  destruct (Mem.storebytes m1 _ _ _) as [m1'|] eqn:Hm1'; [|constructor].
+  assert (vs1 = nil \/ vs1 <> nil) as [Hvs1|Hvs1].
+  { destruct vs1; constructor; congruence. }
+  - subst. inv Hvs.
+    edestruct (Mem.range_perm_storebytes m2 b2 ofs2 nil) as [m2' Hm2'].
+    {
+      intros ofs. simpl. extlia.
+    }
+    rewrite Hm2'.
+    constructor.
+    eexists; split; repeat rstep.
+    erewrite <- (Mem.nextblock_storebytes m1); eauto.
+    erewrite <- (Mem.nextblock_storebytes m2); eauto.
+    constructor; eauto.
+    eapply Mem.storebytes_empty_inject; eauto.
+  - assert (ptr_inject f (b1, ofs1) (b2, ofs2)) as Hptr'.
+    {
+      destruct Hptr as [Hptr|Hptr]; eauto.
+      inversion Hptr as [_ _ [xb1 xofs1 xb2 delta Hb]]; clear Hptr; subst.
+      unfold ptrbits_unsigned.
+      erewrite Mem.address_inject; eauto.
+      apply Mem.storebytes_range_perm in Hm1'.
+      eapply Hm1'.
+      destruct vs1; try congruence.
+      simpl. extlia.
+    }
+    inv Hptr'.
+    edestruct Mem.storebytes_mapped_inject as (m2' & Hm2' & Hm'); eauto. rauto.
+    rewrite Hm2'.
+    repeat (econstructor; eauto); try congruence;
+      erewrite <- Mem.nextblock_storebytes; eauto using Pos.le_refl.
+Qed.
+
+Next Obligation. (* Mem.perm *)
+  intros [f nb1 nb2] m1 m2 Hm _ _ [b1 ofs1 b2 delta Hb] p k H.
+  eapply Mem.perm_inject; eauto.
+Qed.
+
+Next Obligation. (* Mem.valid_block *)
+  intros [f nb1 nb2] m1 m2 Hm b1 b2 [delta Hb].
+  split; intro.
+  - eapply Mem.valid_block_inject_2; eauto.
+  - eapply Mem.valid_block_inject_1; eauto.
+Qed.
+
+Next Obligation. (* Mem.meminj_no_overlap *)
+  destruct H as [f m1 m2 nb1 nb2 Hm Hnb1 Hnb2].
+  eapply Mem.mi_no_overlap; eauto.
+Qed.
+
+Next Obligation. (* representable *)
+  destruct H as [f m1 m2 nb1 nb2 Hm Hnb1 Hnb2].
+  rewrite <- (Ptrofs.unsigned_repr ofs1) by extlia.
+  eapply Mem.mi_representable; eauto.
+  rewrite Ptrofs.unsigned_repr by extlia.
+  assumption.
+Qed.
+
+Next Obligation.
+  destruct H as [f m1 m2 nb1 nb2 Hm Hnb1 Hnb2].
+  eapply Mem.aligned_area_inject; eauto.
+Qed.
+
+Next Obligation. 
+  destruct H as [f m1 m2 nb1 nb2 Hm Hnb1 Hnb2].
+  eapply Mem.disjoint_or_equal_inject; eauto.
+Qed.
+
+Next Obligation. (* perm_inv *)
+  destruct H as [f m1 m2 nb1 nb2 Hm Hnb1 Hnb2].
+  inv H0.
+  eapply Mem.perm_inject_inv; eauto.
+Qed.
+
+Next Obligation. (* nextblock incr *)
+  destruct H0 as (w' & Hw' & Hm').
+  destruct H. inv Hm'. inv Hw'.
+  split; auto.
+Qed.
+
